

# **MATH 109: Homework 5**

*Professor Rabin*

**Nalin Bhardwaj**

A16157819

nibnalin@ucsd.edu

## 1 Problem 4.43

- (a)  $A = \{1, 2\}, B = \{1, 4\}, C = \{1, 5\}$   
 (b)  $A = \{1\}, B = \{2\}, C = \{1, 2\}$   
 (c) Let  $x \in B$ . Two cases arise:

### 1.1 $x \in A$

Then  $x \in A \cap B \implies x \in A \cap C \implies x \in A$  and  $x \in C \implies x \in C$ .

### 1.2 $x \notin A$

Then  $x \in A \cup B \implies x \in A \cup C \implies x \in A$  or  $x \in C \implies x \in C$ .

Therefore,  $B \subseteq C$ .

Similarly, WLOG, let  $x \in C$ . Therefore,  $C \subseteq B$ .

Therefore,  $B = C$ .

## 2 Problem 4.48

$$A = \{n \in \mathbb{Z} : 2|n\}, B = \{n \in \mathbb{Z} : 4|n\}$$

### 2.1 If $n \neq 2k$ for some odd integer $k$ , then $n \notin A - B$

Case 1:  $n = 2k + 1$  for some  $k \in \mathbb{Z}$ .

Then,  $n \notin A \implies n \notin A - B$

Case 2:  $n = 2k$  for some even  $k \in \mathbb{Z}$ .

Then,  $k = 2l$  and  $n = 4l$  for some  $l \in \mathbb{Z}$ .

Therefore,  $n \in A$  and  $n \in B \implies n \notin A - B$ .

### 2.2 If $n = 2k$ for some odd $k$ , then $n \in A - B$

$k = 2l + 1$  for some  $l \in \mathbb{Z}$ . Therefore,  $n = 2(2l + 1) \implies n = 4l + 2$

Since  $2|2(2l + 1)$ ,  $2|n \implies n \in A$  and  $4 \nmid 4l + 2 \implies n \notin B$ . Therefore,  $n \in A - B$ .

## 3 Problem 4.56

Let  $x \in (A - B) \cup (A - C)$ .

WLOG, let  $x \in (A - B)$ .  $x \in (A - B) \implies x \in A$  and  $x \notin B \implies x \notin B \cap C \implies x \in A - (B \cap C)$ .

Therefore,  $(A - B) \cup (A - C) \subseteq A - (B \cap C)$ .

Let  $x \in A - (B \cap C)$ . Therefore,  $x \in A$  and  $x \notin B \cap C$ .

WLOG, let  $x \notin B$ .  $x \notin B \implies x \in A - B \implies x \in (A - B) \cup (A - C)$ .

Therefore,  $A - (B \cap C) \subseteq (A - B) \cup (A - C)$ .

Therefore,  $A - (B \cap C) = (A - B) \cup (A - C)$ .

## 4 Problem 5.4

Let  $n = 2$ .  $\frac{n(n+1)}{2} = 3$  and  $\frac{(n+1)(n+2)}{2} = 6$ . 3 is odd, but 6 is not odd. Hence, the implication is false.

## 5 Problem 5.15

Let  $a$  and  $b$  be odd integers such that  $4|a^2 + b^2$ .

Let  $a^2 + b^2 = 4k_1$ ,  $a = 2k_2 + 1$ ,  $b = 2k_3 + 1$  for some  $k_1, k_2, k_3 \in \mathbb{Z}$ .

$$(2k_2 + 1)^2 + (2k_3 + 1)^2 = 4k_1 \implies 4(k_2^2 + k_2 + k_3^2 + k_3) + 2 = 4k_1 \implies 2 = 4(k_1 - k_2^2 - k_2 + k_3^2 + k_3).$$

Since  $k_1 - k_2^2 - k_2 + k_3^2 + k_3 \in \mathbb{Z}$ , we proved  $4|2$ , which is a contradiction.

## 6 Problem 5.18

Let the irrational number be  $k_1$  and the rational number be  $\frac{p}{q}$  such that  $p, q \in \mathbb{Z}$  and  $q \neq 0$ .

Since  $\frac{p}{q} \neq 0 \implies p \neq 0$ .

Let product  $k_2$  be a rational number.

Then,  $k_2 = \frac{k_1 p}{q}$ . Since  $p \neq 0$ ,  $k_1 = \frac{k_2 q}{p}$ . Since  $\frac{k_2 q}{p}$  is rational, we have shown that  $k_1$  is rational, which is a contradiction.

## 7 Problem 5.20

Let both  $ar + s$  and  $ar - s$  be rational.

Then,  $ar + s = \frac{k_1}{k_2}$  for  $k_1, k_2 \in \mathbb{Z}$  and  $k_2 \neq 0$  and  $ar - s = \frac{k_3}{k_4}$  for  $k_3, k_4 \in \mathbb{Z}$  and  $k_4 \neq 0$ .

Adding,  $2ar = \frac{k_1}{k_2} + \frac{k_3}{k_4} \implies a = \frac{k_1 k_4 + k_2 k_3}{2r k_2 k_4}$  and  $r, k_2, k_4 \neq 0 \implies 2r k_2 k_4 \neq 0$ . Thus, we have shown that  $a$  is rational, which is a contradiction.

## 8 Problem 5.22

Let  $\sqrt{2} + \sqrt{3}$  be rational.

Then,  $\sqrt{2} + \sqrt{3} = \frac{p}{q}$  for  $p, q \in \mathbb{Z}$  and  $q \neq 0$ . Further, since  $\sqrt{2} + \sqrt{3} > 0$ ,  $p \neq 0$ .

$$\begin{aligned} 2 &= \left(\frac{p}{q} - \sqrt{3}\right)^2 \\ 2 &= \frac{p^2}{q^2} + 3 - \frac{2\sqrt{3}p}{q} \\ \frac{p^2}{q^2} + 1 &= \frac{2\sqrt{3}p}{q} \\ \sqrt{3} &= \frac{p^2 + 1}{2pq}, 2pq \neq 0 \end{aligned}$$

By the result of exercise 5.21, we know that  $\sqrt{3}$  is irrational. However, we have shown that  $\sqrt{3}$  is rational, which is a contradiction.

## 9 Problem 5.28

**9.1 Lemma:** For all  $x \in \mathbb{Z}$ , either  $x^2 \equiv 0 \pmod{4}$  or  $x^2 \equiv 1 \pmod{4}$

4 cases arise:

$$\begin{aligned}
x \equiv 0 \pmod{4} &\implies x^2 \equiv 0 \pmod{4} \\
x \equiv 1 \pmod{4} &\implies x^2 \equiv 1 \pmod{4} \\
x \equiv 2 \pmod{4} &\implies x^2 \equiv 0 \pmod{4} \\
x \equiv 3 \pmod{4} &\implies x^2 \equiv 1 \pmod{4}
\end{aligned}$$

## 9.2 Proof

Let there exist integer  $c$  such that for some odd integers  $a$  and  $b$ ,  $a^2 + b^2 = c^2$ .

Then, since  $a$  and  $b$  are odd, the following cases arise:

**9.2.1**  $a \equiv 1 \pmod{4}$  and  $b \equiv 1 \pmod{4}$

$a^2 \equiv 1 \pmod{4}$  and  $b^2 \equiv 1 \pmod{4} \implies a^2 + b^2 \equiv 2 \pmod{4} \implies c^2 \equiv 2 \pmod{4}$ . However, by lemma 10.1, this is a contradiction.

**9.2.2** **WLOG**,  $a \equiv 1 \pmod{4}$  and  $b \equiv 3 \pmod{4}$

$a^2 \equiv 1 \pmod{4}$  and  $b^2 \equiv 1 \pmod{4} \implies a^2 + b^2 \equiv 2 \pmod{4} \implies c^2 \equiv 2 \pmod{4}$ . However, by lemma 10.1, this is a contradiction.

**9.2.3**  $a \equiv 3 \pmod{4}$  and  $b \equiv 3 \pmod{4}$

$a^2 \equiv 1 \pmod{4}$  and  $b^2 \equiv 1 \pmod{4} \implies a^2 + b^2 \equiv 2 \pmod{4} \implies c^2 \equiv 2 \pmod{4}$ . However, by lemma 10.1, this is a contradiction.

Since we arrive at a contradiction in all cases,  $c$  must not be an integer.

## 10 Problem 5.34

Let  $n$  and  $m \in \mathbb{Z}^+$  such that  $m^2 + m + 1 = n^2$ .

Since for any positive integer  $m + 1 > 0$ ,  $m^2 + m + 1 > m^2 \implies n^2 > m^2 \implies n > m$ .

Since  $m^2 + m + 1 = n^2$ , adding  $m > 0$  to the left side,  $m^2 + 2m + 1 > n^2 \implies (m + 1)^2 > n^2 \implies m + 1 > n$ .

Therefore,  $m < n < m + 1$ . Since  $m \in \mathbb{Z}^+$ , we have shown that  $n$  is not an integer (since there are no integers in  $(m, m + 1)$ ), which is a contradiction.

## 11 Problem 5.45

Let there exist nonzero  $a, b$  such that  $\sqrt{a^2 + b^2} = \sqrt[3]{a^3 + b^3}$ .

Then,

$$\begin{aligned}
(a^2 + b^2)^3 &= (a^3 + b^3)^2 \\
a^6 + b^6 + 3a^2b^2(a^2 + b^2) &= a^6 + b^6 + 2a^3b^3 \\
3a^2b^2(a^2 + b^2) &= 2a^3b^3 \\
3(a^2 + b^2) &= 2ab \text{ since } a, b \neq 0 \\
2(a^2 + b^2) + (a - b)^2 &= 0 \\
\frac{(a - b)^2}{a^2 + b^2} &= -2
\end{aligned}$$

Clearly, all nonzero solutions are complex, not real, which is a contradiction.